@prefix : <http://hse.ie/> .
@prefix bibo: <http://purl.org/ontology/bibo/> .
@prefix dcat: <http://www.w3.org/ns/dcat#> .
@prefix dcterms: <http://purl.org/dc/terms/> .
@prefix foaf: <http://xmlns.com/foaf/0.1/> .
@prefix healthdcatap: <http://healthdataportal.eu/ns/health#> .
@prefix owl: <http://www.w3.org/2002/07/owl#> .
@prefix phd: <https://hse.ie/ontology/phd#> .
@prefix phi: <https://hse.ie/ontology/phi#> .
@prefix phpt: <https://hse.ie/terminology/phpt#> .
@prefix rdf: <http://www.w3.org/1999/02/22-rdf-syntax-ns#> .
@prefix rdfs: <http://www.w3.org/2000/01/rdf-schema#> .
@prefix rml: <http://w3id.org/rml/> .
@prefix skos: <http://www.w3.org/2004/02/skos/core#> .
@prefix vann: <http://purl.org/vocab/vann/> .
@prefix xsd: <http://www.w3.org/2001/XMLSchema#> .

# <https://hse.ie/ontology/phd#> a owl:Ontology;
#   dcterms:abstract "The Population Health Datasets Ontology (phd) extends DCAT to describe health datasets and their metadata, including data governance, coding schemes, and applicable legislation for population health planning and analysis.";
#   dcterms:bibliographicCitation "Brennan, R., Liang, J., Chen, H. (2025). Population Health Datasets Ontology. Health Service Executive & ADAPT Centre, UCD. https://hse.ie/ontology/phd";
#   dcterms:contributor "Huan Chen", "Junli Liang, ADAPT UCD";
#   dcterms:creator "Rob Brennan, ADAPT UCD";
#   dcterms:description "An ontology for describing population health datasets and their metadata. It aligns with DCAT, Dublin Core, and related standards, and extends them with additional terms needed for population health planning and analysis.";
#   dcterms:issued "2025-04-25"^^xsd:date;
#   dcterms:modified "2025-09-11"^^xsd:date;
#   dcterms:publisher "Health Service Executive (HSE) & ADAPT Centre, University College Dublin";
#   dcterms:rights "Copyright © 2025 Health Service Executive (HSE) and University College Dublin (UCD).";
#   dcterms:source <https://openreview.net/pdf?id=JMWarUh56o>;
#   dcterms:title "Population Health Datasets Ontology (phd)";
#   bibo:status "Draft";
#   vann:preferredNamespacePrefix "phd";
#   vann:preferredNamespaceUri "https://hse.ie/ontology/phd#";
#   rdfs:comment "An ontology for descibing population health dataset, created during the Older Adult Health and Wellbeing Profile project.";
#   rdfs:label "Population Health Datasets Ontology";
#   rdfs:seeAlso <https://openreview.net/pdf?id=JMWarUh56o>;
#   owl:priorVersion <https://hse.ie/ontology/phd/1.0>;
#   owl:versionInfo "1.0.1";
#   foaf:homepage <https://github.com/hse-ucd/hse-ontology> .

<https://hse.ie/ontology/phi#> a owl:Ontology;
  dcterms:abstract "The Population Health Indicator Ontology (phi) provides a formal vocabulary for describing population health indicators, their definitions, data sources, methodologies, and quality attributes. Developed as part of the Older Adult Health and Wellbeing Profile project.";
  dcterms:bibliographicCitation "Brennan, R., Liang, J., Galadima, H. (2025). Population Health Indicator Ontology. Health Service Executive & ADAPT Centre, UCD. https://hse.ie/ontology/phi";
  dcterms:contributor "Haula Galadima, ADAPT UCD", "Junli Liang, ADAPT UCD", "Rob Brennan, ADAPT UCD";
  dcterms:description "Ontology for modeling population health indicators and datasets based on health DCAT-AP data catalogue";
  dcterms:issued "2025-08-20"^^xsd:date;
  dcterms:license <https://creativecommons.org/licenses/by/4.0/>;
  dcterms:modified "2026-02-03"^^xsd:date;
  dcterms:publisher "Health Service Executive (HSE) & ADAPT Centre, University College Dublin";
  dcterms:rights "Copyright © 2025 Health Service Executive (HSE) and University College Dublin (UCD). This work is licensed under a Creative Commons Attribution 4.0 International License.";
  dcterms:source "OAHP Data Catalogue Schema Proposal v05.13";
  dcterms:title "Population Health Indicator Ontology";
  bibo:status "Draft";
  vann:preferredNamespacePrefix "phi";
  vann:preferredNamespaceUri "https://hse.ie/ontology/phi#";
  rdfs:comment "An ontology for describing population health indicators and datasets, created during the Older Adult Health and Wellbeing Profile project.";
  rdfs:label "Population Health Indicator Ontology";
  rdfs:seeAlso <https://openreview.net/pdf?id=JMWarUh56o>;
  owl:priorVersion <https://hse.ie/ontology/phi/1.0>;
  owl:versionIRI <https://github.com/hse-ucd/hse-ontology/blob/main/phi-ontology.ttl>;
  owl:versionInfo "1.0.1";
  foaf:homepage <https://github.com/hse-ucd/hse-ontology> .

phd:applicableLegislation a owl:ObjectProperty;
  dcterms:contributor "Huan Chen, UCD";
  dcterms:created "2025-04-25"^^xsd:date;
  dcterms:creator "Rob Brennan, ADAPT UCD";
  dcterms:modified "2025-09-11"^^xsd:date;
  dcterms:source "DCAT3";
  rdfs:comment "The legislation that mandates the creation or management of the Dataset.";
  rdfs:domain dcat:Dataset;
  rdfs:label "Applicable Legislation";
  rdfs:range dcat:Resource .

phd:hasCodingScheme a owl:DatatypeProperty;
  dcterms:contributor "Huan Chen, UCD";
  dcterms:created "2025-04-25"^^xsd:date;
  dcterms:creator "Rob Brennan, ADAPT UCD";
  dcterms:modified "2025-09-11"^^xsd:date;
  dcterms:source "DCAT3";
  rdfs:comment "Coding systems in use (ex: ICD-10-CM, DGRs, SNOMED=CT, ...)";
  rdfs:domain dcat:Dataset;
  rdfs:label "Has Coding Scheme";
  rdfs:range xsd:string .

phd:status a owl:DatatypeProperty;
  dcterms:contributor "Huan Chen, UCD";
  dcterms:created "2025-04-25"^^xsd:date;
  dcterms:creator "Rob Brennan, ADAPT UCD";
  dcterms:modified "2025-09-11"^^xsd:date;
  dcterms:source "PHD";
  rdfs:comment "An internal prioritisation process status for the dataset or indicator";
  rdfs:domain dcat:Dataset;
  rdfs:label "Status";
  rdfs:range xsd:string;
  rdfs:seeAlso <https://www.w3.org/TR/vocab-dcat-3/#Property:resource_status> .

phi:Dataset a rdfs:Class;
  dcterms:contributor "Huan Chen, ADAPT UCD";
  dcterms:created "2025-04-25"^^xsd:date;
  dcterms:creator "Rob Brennan, ADAPT UCD";
  dcterms:modified "2025-09-11"^^xsd:date;
  dcterms:source "DCAT3";
  rdfs:comment "Collection of data published or curated by a single agent and available for access or download in one or more serializations or formats";
  rdfs:label "Dataset";
  rdfs:seeAlso <https://www.w3.org/TR/vocab-dcat-3/#Class:Dataset>;
  rdfs:subClassOf <https://www.w3.org/TR/vocab-dcat-3/#Class:Dataset> .

phi:Indicator a rdfs:Class;
  dcterms:created "2025-08-18"^^xsd:date;
  dcterms:creator "Rob Brennan, ADAPT UCD";
  dcterms:modified "2025-08-29"^^xsd:date;
  dcterms:source "OAHP Data Catalogue Schema Proposal v05.13";
  rdfs:comment "A population health indicator that measures specific aspects of health and wellbeing.";
  rdfs:label "Indicator" .

phi:IndicatorGroup a rdfs:Class;
  dcterms:contributor "Junli Liang, ADAPT UCD";
  dcterms:created "2026-02-03"^^xsd:date;
  dcterms:creator "Rob Brennan, ADAPT UCD";
  dcterms:modified "2026-02-03"^^xsd:date;
  dcterms:source "OAHP Data Catalogue Schema Proposal v05.13";
  rdfs:comment "A grouping of related health profile indicators.";
  rdfs:label "Indicator Group" .

phi:accrualPeriodicity a owl:ObjectProperty;
  dcterms:created "2025-08-18"^^xsd:date;
  dcterms:creator "Rob Brennan, ADAPT UCD";
  dcterms:modified "2025-08-29"^^xsd:date;
  dcterms:source "OAHP Data Catalogue Schema Proposal v05.13";
  rdfs:comment "Frequency of indicator update in report, e.g. daily or monthly. This is used with the reporting style to determine the exact frequency and lag of indicator reports.Note that datasets have their own -Frequency of data updates- field to state how often they are updated.";
  rdfs:domain phi:Indicator;
  rdfs:label "Report Frequency";
  rdfs:range skos:Concept;
  rdfs:subPropertyOf dcterms:accrualPeriodicity .

phi:definition a owl:DatatypeProperty;
  dcterms:created "2025-08-18"^^xsd:date;
  dcterms:creator "Rob Brennan, ADAPT UCD";
  dcterms:modified "2025-08-29"^^xsd:date;
  dcterms:source "OAHP Data Catalogue Schema Proposal v05.13";
  rdfs:comment "Technical description of the indicator—what it measures, how it's defined, and any assumptions or limitations in interpretation.";
  rdfs:domain phi:Indicator;
  rdfs:label "Definition";
  rdfs:range xsd:string;
  rdfs:subPropertyOf skos:definition .

phi:denominatorDataElement a owl:DatatypeProperty;
  dcterms:created "2025-08-18"^^xsd:date;
  dcterms:creator "Rob Brennan, ADAPT UCD";
  dcterms:modified "2025-08-29"^^xsd:date;
  dcterms:source "OAHP Data Catalogue Schema Proposal v05.13";
  rdfs:comment "The description of one variable or value that is used in the denominator (if this indicator has one) e.g. population size. Multiple data elements may be present as a list.";
  rdfs:domain phi:Indicator;
  rdfs:label "Denominator Data Element";
  rdfs:range xsd:string .

phi:denominatorSource a owl:ObjectProperty;
  dcterms:created "2025-08-18"^^xsd:date;
  dcterms:creator "Rob Brennan, ADAPT UCD";
  dcterms:modified "2025-08-29"^^xsd:date;
  dcterms:source "OAHP Data Catalogue Schema Proposal v05.13";
  rdfs:comment "Identifier, e.g. URL, for the dataset providing a denominator data element. If there are multiple denominator data elements then multiple datasets must be provided as a list.";
  rdfs:domain phi:Indicator;
  rdfs:label "Denominator Source Dataset";
  rdfs:range dcat:Dataset .

phi:disaggregation a owl:DatatypeProperty;
  dcterms:created "2025-08-18"^^xsd:date;
  dcterms:creator "Rob Brennan, ADAPT UCD";
  dcterms:modified "2025-08-29"^^xsd:date;
  dcterms:source "OAHP Data Catalogue Schema Proposal v05.13";
  rdfs:comment "A list of disaggregation conditions that should be available e.g. male and female";
  rdfs:domain phi:Indicator;
  rdfs:label "Disaggregations";
  rdfs:range xsd:string .

phi:domain a owl:ObjectProperty;
  dcterms:created "2025-08-18"^^xsd:date;
  dcterms:creator "Rob Brennan, ADAPT UCD";
  dcterms:modified "2025-08-29"^^xsd:date;
  dcterms:source "OAHP Data Catalogue Schema Proposal v05.13";
  rdfs:comment "The high-level category the indicator falls under (e.g. Demography).";
  rdfs:domain phi:Indicator;
  rdfs:label "Domain";
  rdfs:range skos:Concept;
  rdfs:seeAlso healthdcatap:healthTheme .

phi:highLowGuidance a owl:DatatypeProperty;
  dcterms:created "2025-08-18"^^xsd:date;
  dcterms:creator "Rob Brennan, ADAPT UCD";
  dcterms:modified "2025-08-29"^^xsd:date;
  dcterms:source "OAHP Data Catalogue Schema Proposal v05.13";
  rdfs:comment "Guidance on how to understand high or low values—whether they suggest good or poor outcomes.";
  rdfs:domain phi:Indicator;
  rdfs:label "High-Low Guidance";
  rdfs:range xsd:string .

phi:historyNote a owl:DatatypeProperty;
  dcterms:created "2025-08-18"^^xsd:date;
  dcterms:creator "Rob Brennan, ADAPT UCD";
  dcterms:modified "2025-08-29"^^xsd:date;
  dcterms:source "OAHP Data Catalogue Schema Proposal v05.13";
  rdfs:comment "Reasons for Inclusion or Exclusion";
  rdfs:domain phi:Indicator;
  rdfs:label "Reasons for Inclusion/Exclusion";
  rdfs:range xsd:string;
  rdfs:subPropertyOf skos:historyNote .

phi:identifier a owl:DatatypeProperty;
  dcterms:created "2025-08-18"^^xsd:date;
  dcterms:creator "Rob Brennan, ADAPT UCD";
  dcterms:modified "2025-08-29"^^xsd:date;
  dcterms:source "OAHP Data Catalogue Schema Proposal v05.13";
  rdfs:comment "The main identifier for the Indicator, e.g. the URI [URL, web link] or other unique identifier in the context of the Catalogue.";
  rdfs:domain phi:Indicator;
  rdfs:label "Indicator ID";
  rdfs:range xsd:anyURI;
  rdfs:subPropertyOf dcterms:identifier .

phi:indicatorType a owl:ObjectProperty;
  dcterms:created "2025-08-18"^^xsd:date;
  dcterms:creator "Rob Brennan, ADAPT UCD";
  dcterms:modified "2025-08-29"^^xsd:date;
  dcterms:source "OAHP Data Catalogue Schema Proposal v05.13";
  rdfs:comment "Specifies if the indicator has both a numerator and a denominator, is coverage, accumulated or qualitative type";
  rdfs:domain phi:Indicator;
  rdfs:label "Indicator Type";
  rdfs:range skos:Concept .

phi:measurementLimitations a owl:DatatypeProperty;
  dcterms:created "2025-08-18"^^xsd:date;
  dcterms:creator "Rob Brennan, ADAPT UCD";
  dcterms:modified "2025-08-29"^^xsd:date;
  dcterms:source "OAHP Data Catalogue Schema Proposal v05.13";
  rdfs:comment "Notes on limitations or uncertainty introduced by how the data are collected or calculated.";
  rdfs:domain phi:Indicator;
  rdfs:label "Measurement Limitations";
  rdfs:range xsd:string .

phi:methodology a owl:DatatypeProperty;
  dcterms:created "2025-08-18"^^xsd:date;
  dcterms:creator "Rob Brennan, ADAPT UCD";
  dcterms:modified "2025-08-29"^^xsd:date;
  dcterms:source "OAHP Data Catalogue Schema Proposal v05.13";
  rdfs:comment "Summary of methods used to calculate the indicator (e.,g statistical technique, smoothing, standardisation, modelling).";
  rdfs:domain phi:Indicator;
  rdfs:label "Methodology";
  rdfs:range xsd:string .

phi:note a owl:DatatypeProperty;
  dcterms:created "2025-08-18"^^xsd:date;
  dcterms:creator "Rob Brennan, ADAPT UCD";
  dcterms:modified "2025-08-29"^^xsd:date;
  dcterms:source "OAHP Data Catalogue Schema Proposal v05.13";
  rdfs:comment "Any additional informal information about the dataset or indicator";
  rdfs:domain phi:Indicator;
  rdfs:label "Notes";
  rdfs:range xsd:string;
  rdfs:subPropertyOf skos:note .

phi:numeratorDataElement a owl:DatatypeProperty;
  dcterms:created "2025-08-18"^^xsd:date;
  dcterms:creator "Rob Brennan, ADAPT UCD";
  dcterms:modified "2025-08-29"^^xsd:date;
  dcterms:source "OAHP Data Catalogue Schema Proposal v05.13";
  rdfs:comment "The description of one variable or value that is used in the numerator e.g. number of deaths. Multiple data elements may be present as a list.";
  rdfs:domain phi:Indicator;
  rdfs:label "Numerator Data Element";
  rdfs:range xsd:string .

phi:numeratorSource a owl:ObjectProperty;
  dcterms:created "2025-08-18"^^xsd:date;
  dcterms:creator "Rob Brennan, ADAPT UCD";
  dcterms:modified "2025-08-29"^^xsd:date;
  dcterms:source "OAHP Data Catalogue Schema Proposal v05.13";
  rdfs:comment "Identifier, e.g. URL, for the dataset providing a numerator data element. If there are multiple numerator data elements then multiple datasets must be provided as a list.";
  rdfs:domain phi:Indicator;
  rdfs:label "Numerator Source Dataset";
  rdfs:range dcat:Dataset .

phi:otherIdentifier a owl:ObjectProperty;
  dcterms:created "2025-08-18"^^xsd:date;
  dcterms:creator "Rob Brennan, ADAPT UCD";
  dcterms:modified "2025-08-29"^^xsd:date;
  dcterms:source "OAHP Data Catalogue Schema Proposal v05.13";
  rdfs:comment "Alternative identifiers for this indicator from other data publishers or coding schemes (as URIs)";
  rdfs:domain phi:Indicator;
  rdfs:label "Other Identifiers";
  rdfs:range rdfs:Resource;
  rdfs:subPropertyOf owl:sameAs .

phi:provenance a owl:DatatypeProperty;
  dcterms:created "2025-08-18"^^xsd:date;
  dcterms:creator "Rob Brennan, ADAPT UCD";
  dcterms:modified "2025-08-29"^^xsd:date;
  dcterms:source "OAHP Data Catalogue Schema Proposal v05.13";
  rdfs:comment "Provenance is information about entities, activities, and people involved in producing an indicator, which can be used to form assessments about its quality, reliability or trustworthiness. For example a description of the source of this indicator, e.g. academic papers or standards, any calculations or adjustments performed on the raw data and any organisations involved in producing or transforming the data.";
  rdfs:domain phi:Indicator;
  rdfs:label "Provenance";
  rdfs:range xsd:string;
  rdfs:subPropertyOf dcterms:provenance .

phi:rationale a owl:DatatypeProperty;
  dcterms:created "2025-08-18"^^xsd:date;
  dcterms:creator "Rob Brennan, ADAPT UCD";
  dcterms:modified "2025-08-29"^^xsd:date;
  dcterms:source "OAHP Data Catalogue Schema Proposal v05.13";
  rdfs:comment "A summary explaining why this indicator matters—its relevance to population health, what it helps to understand, and how it complements other indicators.";
  rdfs:domain phi:Indicator;
  rdfs:label "Rationale";
  rdfs:range xsd:string .

phi:status a owl:ObjectProperty;
  dcterms:created "2025-08-18"^^xsd:date;
  dcterms:creator "Rob Brennan, ADAPT UCD";
  dcterms:modified "2025-08-29"^^xsd:date;
  dcterms:source "OAHP Data Catalogue Schema Proposal v05.13";
  rdfs:comment "An internal prioritisation process status for the dataset or indicator";
  rdfs:domain phi:Indicator;
  rdfs:label "Status";
  rdfs:range skos:Concept;
  rdfs:seeAlso phi:StatusCodes .

phi:subdomain a owl:ObjectProperty;
  dcterms:created "2025-08-18"^^xsd:date;
  dcterms:creator "Rob Brennan, ADAPT UCD";
  dcterms:modified "2025-08-29"^^xsd:date;
  dcterms:source "OAHP Data Catalogue Schema Proposal v05.13";
  rdfs:comment "A more specific category under the domain (e.g. Population numbers).";
  rdfs:domain phi:Indicator;
  rdfs:label "Subdomain";
  rdfs:range skos:Concept;
  rdfs:seeAlso healthdcatap:healthTheme .

phi:title a owl:DatatypeProperty;
  dcterms:created "2025-08-18"^^xsd:date;
  dcterms:creator "Rob Brennan, ADAPT UCD";
  dcterms:modified "2025-08-29"^^xsd:date;
  dcterms:source "OAHP Data Catalogue Schema Proposal v05.13";
  rdfs:comment "Full name of the indicator as used in reports or dashboards.";
  rdfs:domain phi:Indicator;
  rdfs:label "Indicator Title";
  rdfs:range xsd:string;
  rdfs:subPropertyOf dcterms:title .

phi:validityGuidance a owl:DatatypeProperty;
  dcterms:created "2025-08-18"^^xsd:date;
  dcterms:creator "Rob Brennan, ADAPT UCD";
  dcterms:modified "2025-08-29"^^xsd:date;
  dcterms:source "OAHP Data Catalogue Schema Proposal v05.13";
  rdfs:comment "Description of how the indicator might be influenced by other variables or biases, affecting validity.";
  rdfs:domain phi:Indicator;
  rdfs:label "Validity Guidance";
  rdfs:range xsd:string .
